Remove radix
It would be good to support other radices, most notably Decimal, but I'm not really working on that for the most part. There's complexities to the implementation of decimal that I'm not handling, and am not really equipped to handle at this moment in time.
As well, it makes the implementation of the bitformat more complex to prove properties about (removing radix let me get rid of some annoying cast logic, etc.).

Flean/Encoding.lean
@@ -61,18 +61,11 @@ theorem FloatFormat.exponentBits_pos [FloatFormat] :
 
 @[reducible]
 def FloatFormat.bitSize [FloatFormat] : ℕ :=
-  if FloatFormat.radix = Radix.Binary then
-    -- 1 for the sign bit, F.prec - 1 for the significand, and F.prec for the exponent
-    -- we can skip 1 bit because we don't need to represent the leading 1/0 in the significand
-    FloatFormat.signBits + FloatFormat.exponentBits + FloatFormat.significandBits
-  else
-    -- TODO: How do you compute this for the decimal format, or other cases?
-    -- Should we have this be in the units that the radix is defined in, instead of general bits?
-    0
+  -- 1 for the sign bit, F.prec - 1 for the significand, and F.prec for the exponent
+  -- we can skip 1 bit because we don't need to represent the leading 1/0 in the significand
+  FloatFormat.signBits + FloatFormat.exponentBits + FloatFormat.significandBits
 
-def FloatFormat.bitSize_eq_binary [FloatFormat] (h : FloatFormat.radix = Radix.Binary) :
-  FloatFormat.bitSize = FloatFormat.signBits + FloatFormat.exponentBits + FloatFormat.significandBits := by
-  simp only [FloatFormat.bitSize, h, ↓reduceIte]
+def FloatFormat.bitSize_eq [FloatFormat] : FloatFormat.bitSize = FloatFormat.signBits + FloatFormat.exponentBits + FloatFormat.significandBits := rfl
 
 /-- Added to the exponent to make the biased exponent, a non-negative number -/
 @[reducible]
@@ -164,11 +157,8 @@ namespace FloatBits
 variable [FloatFormat]
 
 def mk' (sign : BitVec FloatFormat.signBits) (exponent : BitVec FloatFormat.exponentBits) (significand : BitVec FloatFormat.significandBits) : FloatBits :=
-  if hr : FloatFormat.radix = Radix.Binary then
-    let b := sign ++ exponent ++ significand
-    {b := BitVec.cast (FloatFormat.bitSize_eq_binary hr).symm b}
-  else
-    {b := 0}
+  let b := sign ++ exponent ++ significand
+  {b := BitVec.cast FloatFormat.bitSize_eq.symm b}
 
 def ext1 (b : FloatBits) (c : BitVec FloatFormat.bitSize) : b = ⟨c⟩ ↔ b.b = c := by
   constructor
@@ -183,7 +173,7 @@ def toBitsTriple (b : FloatBits) : FloatBitsTriple :=
   let significand := b.extractLsb' 0 FloatFormat.significandBits
   {sign := sign, exponent := exponent, significand := significand}
 
-theorem appendToBitsTriple_eq (hr : FloatFormat.radix = Radix.Binary) (t : FloatBitsTriple) : (b : FloatBits) → b.toBitsTriple = t → b = FloatBits.mk' t.sign t.exponent t.significand := by
+theorem appendToBitsTriple_eq (t : FloatBitsTriple) : (b : FloatBits) → b.toBitsTriple = t → b = FloatBits.mk' t.sign t.exponent t.significand := by
   intro b h
   unfold FloatBits.toBitsTriple at h
   lift_lets at h
@@ -193,19 +183,28 @@ theorem appendToBitsTriple_eq (hr : FloatFormat.radix = Radix.Binary) (t : Float
 
   unfold FloatBits.mk'
   unfold FloatFormat.bitSize
-  split_ifs
   apply (ext1 _ _).mpr
 
   rw [show 1 + FloatFormat.exponentBits + FloatFormat.significandBits - 1 = FloatFormat.significandBits + FloatFormat.exponentBits by omega]
   rw [show 1 + FloatFormat.exponentBits + FloatFormat.significandBits - FloatFormat.exponentBits - 1 = FloatFormat.significandBits by omega]
 
-  let bb' : BitVec (FloatFormat.signBits + FloatFormat.exponentBits + FloatFormat.significandBits) := BitVec.cast (FloatFormat.bitSize_eq_binary hr) b.b
+  let bb' : BitVec (FloatFormat.signBits + FloatFormat.exponentBits + FloatFormat.significandBits) := BitVec.cast FloatFormat.bitSize_eq.symm b.b
   have bz := @BitVec.extractBreakup₃ FloatFormat.signBits FloatFormat.exponentBits FloatFormat.significandBits bb'
   rw [add_comm FloatFormat.exponentBits] at bz
 
-  rw [BitVec.cast_eq_swap (FloatFormat.bitSize_eq_binary hr)]
-  repeat rw [← BitVec.extractLsb'_cast (FloatFormat.bitSize_eq_binary hr)]
+  rw [BitVec.cast_eq_swap (FloatFormat.bitSize_eq)]
   unfold_let bb' at bz
+  -- We run into the issue that it will just nest the cast inside the cast when we apply it again, is there a better way?
+  rw [← BitVec.extractLsb'_cast (FloatFormat.bitSize_eq)]
+  conv =>
+    rhs
+    rhs
+    rw [← BitVec.extractLsb'_cast (FloatFormat.bitSize_eq)]
+  conv =>
+    rhs
+    lhs
+    rhs
+    rw [← BitVec.extractLsb'_cast (FloatFormat.bitSize_eq)]
   rw [bz]
 
 def toValueTriple (b : FloatBits) : Bool × ℤ × ℤ :=
@@ -378,28 +377,15 @@ theorem disj (b : FloatBits) : (Xor' (Xor' b.isNaN b.isInfinite) b.isFinite) := 
 -- TODO: disj between nan, infinite, normal finite, subnormal finite and zero
 
 /-- Constructing a `FloatBitsTriple` from a `FloatBits` made by `(s, E, T)` will yield the same `(s, E, T)` -/
-theorem construct_triple_eq_BitsTriple (hr : FloatFormat.radix = Radix.Binary) (s : BitVec FloatFormat.signBits) (E : BitVec FloatFormat.exponentBits) (T : BitVec FloatFormat.significandBits) :
+theorem construct_triple_eq_BitsTriple (s : BitVec FloatFormat.signBits) (E : BitVec FloatFormat.exponentBits) (T : BitVec FloatFormat.significandBits) :
   (FloatBits.mk' s E T).toBitsTriple.sign = s ∧ (FloatBits.mk' s E T).toBitsTriple.exponent = E ∧ (FloatBits.mk' s E T).toBitsTriple.significand = T := by
   unfold FloatBits.mk' FloatBits.toBitsTriple
   lift_lets
   norm_num
-  split_ifs
   unfold FloatFormat.signBits
   -- Is there no way to use omega to simplify?
   rw [show 1 + FloatFormat.exponentBits + FloatFormat.significandBits - FloatFormat.exponentBits - 1 = FloatFormat.significandBits by omega]
   rw [show 1 + FloatFormat.exponentBits + FloatFormat.significandBits - 1 = FloatFormat.significandBits + FloatFormat.exponentBits by omega]
-
-  have kh : 1 + FloatFormat.exponentBits + FloatFormat.significandBits = FloatFormat.bitSize := by
-    unfold FloatFormat.bitSize
-    split_ifs
-    linarith
-
-  -- Simplify the casts out
-  have k0 := λ (off size) => BitVec.extractLsb'_cast kh off size (s ++ E ++ T)
-  have kS := k0 (FloatFormat.significandBits + FloatFormat.exponentBits) FloatFormat.signBits
-  have kE := k0 FloatFormat.significandBits FloatFormat.exponentBits
-  have kT := k0 0 FloatFormat.significandBits
-  rw [kE, kT, kS]
 
   have jS := @BitVec.extractAppend_third₃ FloatFormat.signBits FloatFormat.exponentBits FloatFormat.significandBits s E T
   have jE := @BitVec.extractAppend_second₃ FloatFormat.signBits FloatFormat.exponentBits FloatFormat.significandBits s E T
@@ -407,41 +393,36 @@ theorem construct_triple_eq_BitsTriple (hr : FloatFormat.radix = Radix.Binary) (
   rw [jE, jT, jS]
   repeat1 constructor
 
-theorem construct_sign_eq_BitsTriple (hr : FloatFormat.radix = Radix.Binary) (s : BitVec FloatFormat.signBits) (E : BitVec FloatFormat.exponentBits) (T : BitVec FloatFormat.significandBits) :
-  (FloatBits.mk' s E T).toBitsTriple.sign = s := (construct_triple_eq_BitsTriple hr s E T).1
+theorem construct_sign_eq_BitsTriple (s : BitVec FloatFormat.signBits) (E : BitVec FloatFormat.exponentBits) (T : BitVec FloatFormat.significandBits) :
+  (FloatBits.mk' s E T).toBitsTriple.sign = s := (construct_triple_eq_BitsTriple s E T).1
 
-theorem construct_exponent_eq_BitsTriple (hr : FloatFormat.radix = Radix.Binary) (s : BitVec FloatFormat.signBits) (E : BitVec FloatFormat.exponentBits) (T : BitVec FloatFormat.significandBits) :
-  (FloatBits.mk' s E T).toBitsTriple.exponent = E := (construct_triple_eq_BitsTriple hr s E T).2.1
+theorem construct_exponent_eq_BitsTriple (s : BitVec FloatFormat.signBits) (E : BitVec FloatFormat.exponentBits) (T : BitVec FloatFormat.significandBits) :
+  (FloatBits.mk' s E T).toBitsTriple.exponent = E := (construct_triple_eq_BitsTriple s E T).2.1
 
-theorem construct_significand_eq_BitsTriple (hr : FloatFormat.radix = Radix.Binary) (s : BitVec FloatFormat.signBits) (E : BitVec FloatFormat.exponentBits) (T : BitVec FloatFormat.significandBits) :
-  (FloatBits.mk' s E T).toBitsTriple.significand = T := (construct_triple_eq_BitsTriple hr s E T).2.2
+theorem construct_significand_eq_BitsTriple (s : BitVec FloatFormat.signBits) (E : BitVec FloatFormat.exponentBits) (T : BitVec FloatFormat.significandBits) :
+  (FloatBits.mk' s E T).toBitsTriple.significand = T := (construct_triple_eq_BitsTriple s E T).2.2
 
 /-- Get the bit representation of an infinite float. -/
 def infinite (b : Bool) : FloatBits :=
-  if FloatFormat.radix = Radix.Binary then
-    let sign := BitVec.ofBool b
-    let significand := BitVec.ofNat FloatFormat.significandBits 0
-    let exponent := BitVec.allOnes FloatFormat.exponentBits
-    FloatBits.mk' sign exponent significand
-  else
-    FloatBits.mk 0
+  let sign := BitVec.ofBool b
+  let significand := BitVec.ofNat FloatFormat.significandBits 0
+  let exponent := BitVec.allOnes FloatFormat.exponentBits
+  FloatBits.mk' sign exponent significand
 
 /-- Constructing an infinite float will yield an infinite float. -/
-theorem infinite_isInfinite (hr : FloatFormat.radix = Radix.Binary) (b : Bool) :
+theorem infinite_isInfinite (b : Bool) :
   (infinite b).isInfinite := by
   unfold FloatBits.isInfinite FloatBits.isExponentAllOnes FloatBits.isTSignificandZero FloatBits.infinite
-  split_ifs
   norm_num
   rw [BitVec.ofNat_eq_ofNat]
   constructor
-  · rw [construct_exponent_eq_BitsTriple hr]
-  · rw [construct_significand_eq_BitsTriple hr]
+  · rw [construct_exponent_eq_BitsTriple]
+  · rw [construct_significand_eq_BitsTriple]
 
-theorem isInfinite_val (b : FloatBits) (hr : FloatFormat.radix = Radix.Binary) : b.isInfinite ↔ b = FloatBits.infinite true ∨ b = FloatBits.infinite false := by
+theorem isInfinite_val (b : FloatBits) : b.isInfinite ↔ b = FloatBits.infinite true ∨ b = FloatBits.infinite false := by
   constructor
   · unfold FloatBits.isInfinite FloatBits.infinite
     intro ⟨he, hsig⟩
-    split_ifs
     norm_num
     cases (BitVec.one_or b.toBitsTriple.sign)
     <;> {
@@ -452,7 +433,7 @@ theorem isInfinite_val (b : FloatBits) (hr : FloatFormat.radix = Radix.Binary) :
         <;> norm_num
         assumption; assumption
 
-      have k := FloatBits.appendToBitsTriple_eq hr _ b h1
+      have k := FloatBits.appendToBitsTriple_eq _ b h1
       rw [h0] at k
       simp only [k, BitVec.ofNat_eq_ofNat, or_true, true_or]
     }
@@ -461,28 +442,24 @@ theorem isInfinite_val (b : FloatBits) (hr : FloatFormat.radix = Radix.Binary) :
     <;> {
       intro hv
       rw [hv]
-      apply infinite_isInfinite hr
+      apply infinite_isInfinite
     }
 
 /-- Construct a NaN with the given sign bit and significand. -/
 def NaN (sign : Bool) (T : BitVec FloatFormat.significandBits) (_hT : T ≠ 0): FloatBits :=
-  if FloatFormat.radix = Radix.Binary then
-    let sign := BitVec.ofBool sign
-    let significand := T
-    let exponent := BitVec.allOnes FloatFormat.exponentBits
-    FloatBits.mk' sign exponent significand
-  else
-    FloatBits.mk 0
+  let sign := BitVec.ofBool sign
+  let significand := T
+  let exponent := BitVec.allOnes FloatFormat.exponentBits
+  FloatBits.mk' sign exponent significand
 
 /-- Constructing a NaN will yield a NaN. -/
-theorem NaN_isNaN (hr : FloatFormat.radix = Radix.Binary) (sign : Bool) (T : BitVec FloatFormat.significandBits) (hT : T ≠ 0):
+theorem NaN_isNaN (sign : Bool) (T : BitVec FloatFormat.significandBits) (hT : T ≠ 0):
   (NaN sign T hT).isNaN := by
   unfold FloatBits.isNaN FloatBits.isExponentAllOnes FloatBits.NaN
-  split_ifs
   norm_num
   constructor
-  · rw [construct_exponent_eq_BitsTriple hr]
-  · rw [construct_significand_eq_BitsTriple hr]
+  · rw [construct_exponent_eq_BitsTriple]
+  · rw [construct_significand_eq_BitsTriple]
     trivial
 
 -- TODO: proof for finite floats that we are able to fit the values into the bits, that is, `.toNat` on the fields will return the original value
@@ -491,19 +468,16 @@ def sigToTrailing (m : ℕ) := m &&& (2^FloatFormat.significandBits - 1)
 
 /-- Construct a finite float from the sign, exponent, and integral significand. -/
 def finite (s : Bool) (e : ℤ) (m : ℕ) : FloatBits :=
-  if FloatFormat.radix = Radix.Binary then
-    -- Biased exponent
-    let E := e + FloatFormat.exponentBias
-    let E := E.toNat
-    -- TODO: we aren't doing this dependent on the Nat which likely makes it harder to infer that it is necessary
-    -- Trailing significand. We can cut off the leading bit because that is entangled with the exponent's value.
-    let T := sigToTrailing m
-    let sign := BitVec.ofBool s
-    let significand := BitVec.ofNat FloatFormat.significandBits T
-    let exponent := BitVec.ofNat FloatFormat.exponentBits E
-    FloatBits.mk' sign exponent significand
-  else
-    FloatBits.mk 0
+  -- Biased exponent
+  let E := e + FloatFormat.exponentBias
+  let E := E.toNat
+  -- TODO: we aren't doing this dependent on the Nat which likely makes it harder to infer that it is necessary
+  -- Trailing significand. We can cut off the leading bit because that is entangled with the exponent's value.
+  let T := sigToTrailing m
+  let sign := BitVec.ofBool s
+  let significand := BitVec.ofNat FloatFormat.significandBits T
+  let exponent := BitVec.ofNat FloatFormat.exponentBits E
+  FloatBits.mk' sign exponent significand
 
 -- TODO: trailing to significand, takes E as well
 
